refinedVST/typing/base.v
@@ -3,11 +3,11 @@ From VST.lithium Require Export syntax definitions.
 From compcert.cfrontend Require Export Ctypes.
 From VST.sepcomp Require Export extspec.
 Set Warnings "-notation-overridden,-custom-entry-overridden,-hiding-delimiting-key".
-From VST.veric Require Export Clight_base expr valid_pointer Cop2 Clight_Cop2 val_lemmas res_predicates mpred seplog tycontext lifting_expr lifting mapsto_memory_block.
-Set Warnings "notation-overridden,custom-entry-overridden,hiding-delimiting-key".
+From VST.veric Require Export Clight_base expr valid_pointer Cop2 Clight_Cop2 val_lemmas res_predicates mpred seplog tycontext lifting mapsto_memory_block.
 From VST.floyd Require Export functional_base base nested_field_lemmas.
-Export Address.
+From VST.veric Require Export lifting_expr.
 From VST Require Export shared.dshare.
+Set Warnings "notation-overridden,custom-entry-overridden,hiding-delimiting-key".
 
 Class CoPsetFact (P : Prop) : Prop := copset_fact : P.
 (* clear for performance reasons as there can be many hypothesis and they should not be needed for the goals which occur *)
